Progress

examples/Queue.v
@@ -12,7 +12,8 @@ From TICL Require Import
   ICTree.Logic.CanStep
   ICTree.Interp.State
   ICTree.Events.State
-  ICTree.Events.Writer.
+  ICTree.Events.Writer
+  Lang.StImpQ.
 
 From ExtLib Require Export
   Structures.MonadState
@@ -31,52 +32,13 @@ Local Open Scope ictree_scope.
 Local Open Scope ticl_scope.
 Local Open Scope list_scope.
 
-Variant queueE (S: Type): Type :=
-  | Push (s: S)
-  | Pop.
-
-Arguments Push {S} s.
-Arguments Pop {S}.
-
-Global Instance encode_queueE{S}: Encode (queueE S) :=
-    fun e => match e with
-          | Push s => unit
-          | Pop => option S
-          end.
-
-Definition push {S}: S -> ictree (queueE S) unit :=
-  fun (s: S) => @ICtree.trigger (queueE S) (queueE S) _ _ (ReSum_refl) (ReSumRet_refl) (Push s).
-
-Definition pop {S}: ictree (queueE S) (option S) :=
-  ICtree.trigger Pop.
-
-Arguments push /.
-Arguments pop /.
-
-Section QueueEx.
-  Context {T: Type} {HDec: RelDec (@eq T)} {HCor: RelDec_Correct HDec}.
+Module Drain.
+  Include StImpQ.
   Infix "=?" := (rel_dec) (at level 75).
 
-  (* Queue instrumented semantics *)
-  Definition h_queueE: queueE T ~> stateT (list T) (ictreeW T) :=
-    fun e =>
-      mkStateT (fun q =>
-                 match e return ictreeW T (encode e * list T) with
-                 | Push v => Ret (tt, q ++ [v])
-                 | Pop => match q with
-                         | nil => Ret (None, nil)
-                         | h :: ts =>
-                             log h ;; (* Instrument the head of the queue [h] *)
-                             Ret (Some h, ts)
-                         end
-                 end).
-
-  Local Open Scope ictree_scope.
   (* Ex1: Drain a queue until there is nothing left *)
-  Definition drain: ictree (queueE T) unit :=
-    loop
-      (x <- pop ;;
-       continue).
+  Definition drain: CProg unit :=
+    CUntilNone CPop.
 
   Lemma list_app_nil: forall (s: T) hs,
       ~ [] = hs ++ [s].
@@ -90,16 +52,14 @@ Section QueueEx.
       end.
   Proof. destruct hs; intros; cbn in *; inv H; auto. Qed.
 
-  (*| Eventually we get [nl] (needle) to show up
-    in the instrumentation. |*)
+  (*| Eventually we get [nl] (needle) to show up |*)
   Example drain_af_pop: forall (nl: T) (q: list T),
-      <( {interp_state h_queueE drain (q ++ [nl])}, Pure |=
-         AF visW {fun w => w = nl })>.
+      <[ {instr_prog drain (q ++ [nl])}, Pure |= AF finishW= tt [] nl ]>.
   Proof with eauto with ticl.
-    intros.
-    apply aul_state_iter_nat
-      with (f:=fun 'tt l _ => List.length l)
-           (Ri:=fun 'tt l w =>
+    intros; unfold drain.
+    eapply aur_qprog_termination
+      with (f:=fun q => List.length q)
+           (Ri:=fun l w =>
                   match w with
                   | Obs (Log s') tt =>
                       match l with
@@ -108,7 +68,7 @@ Section QueueEx.
                       end
                   | _ => exists hs, l = hs ++ [nl]
                   end)...
-    intros [] l w Hd Hw.
+    intros l w Hw Hd.
     destruct l as [|h ts] eqn:Hl; subst.
     - (* l = [] *)
       inv Hd.
@@ -116,52 +76,42 @@ Section QueueEx.
         destruct Hw.
         now apply list_app_nil in H.
       + (* w = Obs e v *)
-        destruct e, v. subst.
-        left.
-        cleft.
-        now csplit.
+        destruct e, v; subst.
+        exists None, [], (Obs (Log t) tt); intuition.
+        * cleft.
+          apply axr_pop_nil...
+        * apply axr_ret...
+          econstructor.
+          exists tt; intuition.
     - (* l = h :: ts *)
-      right.
-      eapply aur_state_bind_r_eq.
-      + rewrite (@interp_state_trigger _ _ _ _ _ _ Pop _); cbn.
-        rewrite bind_bind.
-        eapply afr_log...
-        rewrite bind_ret_l, sb_guard.
-        cleft.
-        apply axr_ret...
-      + cbn.
-        rewrite interp_state_ret.
-        cleft.
-        apply axr_ret...
-        exists tt; intuition.
-        cbn.
-        * inv Hd.
-          -- destruct Hw.
-             apply list_app_cons in H.
-             destruct x; intuition; subst...
-             destruct x; intuition; cbn.
-             ++ now (exists []).
-             ++ now (exists (t0 ::x)).
-          -- destruct e, v, Hw.
-             apply list_app_cons in H.
-             destruct x; intuition; subst...
-             destruct x; intuition; cbn.
-             ++ now (exists []).
-             ++ now (exists (t1 ::x)).
+      exists (Some h), ts, (Obs (Log h) tt); intuition.
+      + apply aur_pop_cons...
+        csplit...
+      + inv Hd.
+        * destruct Hw.
+          apply list_app_cons in H.
+          destruct x; intuition; subst...
+          destruct x; intuition; cbn.
+          -- now (exists []).
+          -- now (exists (t0 ::x)).
+        * destruct e, v, Hw.
+          apply list_app_cons in H.
+          destruct x; intuition; subst...
+          destruct x; intuition; cbn.
+          -- now (exists []).
+          -- now (exists (t1 ::x)).
   Qed.
   Print Assumptions drain_af_pop.
 
   (* Ex2: Rotate a queue (pop an element from head, add it to tail) *)
-  Definition rotate: ictree (queueE T) unit :=
-    loop
-      (x <- pop ;;
-       match x with
-       | Some v =>
-           push v;;
-           continue
-       | None => continue
-       end).
-
+  Definition rotate: CProg unit :=
+    CUntilNone
+      (CBind CPop
+         (fun opt =>
+            CBind
+              (CIfSome opt (fun x => CPush x))
+              (fun 'tt => CRet (Some tt)))).
+              
   (* Element [t] appears unique in [l] in some position *)
   Fixpoint find(t: T) (l: list T): option nat :=
     match l with
@@ -186,11 +136,13 @@ Section QueueEx.
     induction ts.
     - exists 0; cbn.
       rewrite rel_dec_eq_true...
+      typeclasses eauto.
     - destruct IHts.
       destruct (a =? nl) eqn:Hnl.
       + rewrite rel_dec_correct in Hnl; subst.
         exists 0; cbn.
         rewrite rel_dec_eq_true...
+        typeclasses eauto.
       + exists (S x); cbn.
         rewrite Hnl, H.
         reflexivity.
@@ -219,37 +171,34 @@ Section QueueEx.
 
   Theorem rotate_agaf_pop: forall q i,
       find nl q = Some i ->
-      <( {interp_state h_queueE rotate q}, Pure |=
-                       AG AF visW {fun h => h = nl} )>.
+      <( {instr_prog rotate q}, Pure |= AG AF visW {fun h => h = nl} )>.
   Proof with eauto with ticl.
     intros.
-    unfold rotate, forever, Classes.iter, MonadIter_ictree.
-    apply ag_state_iter with
-      (R:= fun 'tt q w => exists h ts, q = h :: ts /\ (h = nl \/ (h <> nl /\ exists i, find nl ts = Some i)))...
+    unfold rotate; cbn. 
+    apply ag_qprog_invariance with
+      (R:= fun q w => exists h ts, q = h :: ts /\ (h = nl \/ (h <> nl /\ exists i, find nl ts = Some i)))...
     - destruct q; try solve [ inv H ].
       exists t, q; intuition.
       rewrite unfold_find_hd in H.
       destruct (t =? nl) eqn:Hnl; inv H.
-      + apply rel_dec_correct in Hnl.
+      + rewrite rel_dec_correct in Hnl.
         left...
       + right.
         destruct (find nl q) eqn:Hq, i; inv H1.
         apply neg_rel_dec_correct in Hnl; split...
     - clear H q.
-      unfold Classes.iter, MonadIter_ictree.
-      intros [] q w Hd (h & ts & -> & [-> | (Hnl & Hi)]).
+      intros q w (h & ts & -> & [-> | (Hnl & Hi)]) Hd.
       + (* t = nl *)
         split.
         * (* iter |= AF *)
-          rewrite interp_state_unfold_iter.
-          apply ticll_bind_l.
-          rewrite interp_state_bind.
-          setoid_rewrite (@interp_state_trigger _ _ _ _ _ _ Pop _); cbn.
-          rewrite ?bind_bind.
-          apply afl_log...
-          cleft.
-          csplit...
+          apply aul_qprog_until_now.
+          eapply aul_qprog_bind.
+          -- eapply aur_pop_cons...
+             csplit...
+          -- cleft.
+             apply ticll_vis...
         * (* body variant/invariant *)
+          eapply aur_qprog_bind.
           rewrite interp_state_bind.
           setoid_rewrite (@interp_state_trigger _ _ _ _ _ _ Pop _); cbn.
           rewrite ?bind_bind.
